

Problem 1: Orthogonal Complement of a Subspace

Solution

(a) Suppose $x_1, x_2 \in \mathcal{V}^\perp$, for any $y \in \mathcal{V}$

$$(x_1 + x_2)^T y = (x_1^T + x_2^T)y = x_1^T y + x_2^T y = 0$$

For any $\alpha \in \mathbb{R}$,

$$(\alpha x_1)^T y = \alpha x_1^T y = 0$$

Hence \mathcal{V}^\perp is a subspace of \mathbb{R}^n .

(b) Because $\mathcal{V} = \text{span}(v_1, v_2, \dots, v_k)$, for any $y \in \mathcal{V}$,

$$y = \sum_{i=1}^k \alpha_i v_i = \begin{bmatrix} v_1 & v_2 & \dots & v_k \end{bmatrix} \begin{bmatrix} \alpha_1 \\ \alpha_2 \\ \vdots \\ \alpha_k \end{bmatrix}, \text{ where } \alpha_1, \dots, \alpha_k \in \mathbb{R}$$

Hence $\mathcal{V} = R(A)$.

For any $y \in \mathcal{V}$,

$$\begin{aligned} x^T y &= x^T A \begin{bmatrix} \alpha_1 \\ \alpha_2 \\ \vdots \\ \alpha_k \end{bmatrix} = 0, \text{ where } \alpha_1, \dots, \alpha_k \in \mathbb{R} \\ &\Rightarrow \left(A \begin{bmatrix} \alpha_1 \\ \alpha_2 \\ \vdots \\ \alpha_k \end{bmatrix} \right)^T x = 0 \\ &\Rightarrow [\alpha_1 \quad \alpha_2 \quad \dots \quad \alpha_k] A^T x = 0 \\ &\Rightarrow A^T x = 0 \end{aligned}$$

Hence $\mathcal{V}^\perp = N(A^T)$.

(c) $(\mathcal{V}^\perp)^\perp$ can be represented as the following:

$$(\mathcal{V}^\perp)^\perp = \{y \in \mathbb{R}^n : y^T x = 0, \forall x \in \mathcal{V}^\perp\}$$

Meanwhile, for any $x \in \mathcal{V}^\perp$,

$$x^T y = 0, \forall y \in \mathcal{V} \Rightarrow y^T x = 0, \forall y \in \mathcal{V}$$

Hence $(\mathcal{V}^\perp)^\perp = \mathcal{V}$

(d)

$$\dim(\mathcal{V}) = \dim[R(A)] = \text{rank}(A) = \text{rank}(A^T) = \dim[R(A^T)]$$

Meanwhile

$$\dim(\mathcal{V}^\perp) = \dim[N(A^T)]$$

Hence

$$\dim(\mathcal{V}) + \dim(\mathcal{V}^\perp) = \dim[R(A^T)] + \dim[N(A^T)] = n$$

(e) According to the definition,

$$\mathcal{W}^\perp = \{x_2 \in \mathbb{R}^n : x_2^T y_2 = 0, \forall y_2 \in \mathcal{W}\}$$

For any $y_1 \in \mathcal{V}$. Because $\mathcal{V} \subseteq \mathcal{W}$, $y_1 \in \mathcal{W}$, hence

$$x_2^T y_1 = 0 \Rightarrow x_2 \in \mathcal{V}^\perp$$

Hence $\mathcal{V} \subseteq \mathcal{W}$ for another subspace \mathcal{W} implies $\mathcal{W}^\perp \subseteq \mathcal{V}^\perp$

(f) Suppose v is the projection of x onto subspace \mathcal{V} . Then

$$\langle x - v, y \rangle = 0, \forall y \in \mathcal{V}$$

$$\Rightarrow y^T(x - v) = 0, \forall y \in \mathcal{V}$$

$$\Rightarrow (x - v)^T y = 0, \forall y \in \mathcal{V}$$

So $(x - v) \in \mathcal{V}^\perp$. Suppose there is a vector v^\perp , S.T.

$$x - v = v^\perp$$

$$\Rightarrow x = v + v^\perp$$

Meanwhile, because v is the projection of x onto subspace \mathcal{V} , v must be unique and thus v^\perp is also unique. Hence any $x \in \mathbb{R}^n$ could be expressed uniquely as $x = v + v^\perp$.

Problem 2: Rank of a Product

Solution Suppose matrix A is

$$\begin{bmatrix} a_1^T \\ a_2^T \\ a_3^T \\ a_4^T \end{bmatrix}$$

$$\Rightarrow AB = [B^T a_1 \quad B^T a_2 \quad B^T a_3 \quad B^T a_4]$$

Because $\text{Rank}(A) = 2$, there should be $\alpha_1, \alpha_2 \in \mathbb{R}$ such that $a_3 = \alpha_1 a_1 + \alpha_2 a_2$. Hence $B^T a_3 = \alpha_1 B^T a_1 + \alpha_2 B^T a_2$. The same could be show that $B^T a_4 = \beta_1 B^T a_1 + \beta_2 B^T a_2$. Hence there is two linear independent vectors at most in a_1, a_2, a_3, a_4 . Hence

$$\text{rank}(AB) \leq 2$$

The folloing will show that $B^T a_1$ and $B^T a_2$ is linear independent. Suppose $\alpha_1, \alpha_2 \in \mathbb{R}$. a_1 and a_2 are linear independent.

$$\alpha_1 B^T a_1 + \alpha_2 B^T a_2 = 0 \Rightarrow B^T(\alpha_1 a_1 + \alpha_2 a_2) = 0$$

Because B is full-rank, so $\dim(N(B^T)) = 3 - 3 = 0$. Hence $N(B^T) = 0$ and $\alpha_1 a_1 + \alpha_2 a_2 = 0$. Because a_1 and a_2 are linear independent, $\alpha_1 = \alpha_2 = 0$. So $B^T a_1$ and $B^T a_2$ are linear independent. Hence

$$\text{rank}(AB) = \text{rank}(B^T A^T) \geq 2$$

Hence $r_{\min} = r_{\max} = 2$. The following is the special case:

$$A = \begin{bmatrix} 1 & 0 & 0 \\ 0 & 1 & 0 \\ 0 & 0 & 0 \\ 0 & 0 & 0 \end{bmatrix}$$

$$B = \begin{bmatrix} 1 & 0 & 0 \\ 0 & 1 & 0 \\ 0 & 0 & 1 \end{bmatrix}$$

Problem 3: An Inequality for Orthonormal Matrices

Solution

$$\|U^T x\|_2 \leq \|x\|_2 \Leftrightarrow \|U^T x\|_2^2 \leq \|x\|_2^2 \Leftrightarrow (U^T x)^T U^T x \leq x^T x$$

Hence we only have to show that

$$x^T x - x^T u u^T x \geq 0$$

$$\Rightarrow x^T (I - u u^T) x \geq 0$$

Suppose $v = (I - u u^T)x$,

$$\begin{aligned} v^T v &= (I - u u^T)^T (I - u u^T) x^T x \\ &= (I - u u^T) (I - u u^T) x^T x \\ &= I - u u^T - u u^T + u u^T u u^T x^T x \\ &= I - u u^T - u u^T + u I u^T x^T x \\ &= I - u u^T x^T x \\ &= v^T v \end{aligned}$$

Hence

$$x^T(I - uu^T)x = x^Tvx = x^Tv^Tvx = \langle vx, vx \rangle$$

Because $\langle vx, vx \rangle \geq 0$, hence $x^T(I - uu^T)x \geq 0$. So $\|U^Tx\|_2 \leq \|x\|_2$ is valid.

Problem 4: Householder Reflections

Solution

(a)

$$\begin{aligned} QQ^T &= (I - 2uu^T)(I - 2uu^T)^T \\ &= (I - 2uu^T)^T - 2uu^T(I - 2uu^T)^T \\ &= I - 2uu^T - 2uu^T + 4uu^Tuu^T \\ &= I - 4uu^T + 4u(u^Tu)u^T \end{aligned}$$

Because u is unit vector, $u^Tu = \|u\|^2 = 1$. Hence $u(u^Tu)u^T = uu^T$, so $QQ^T = I$. Therefore, Q is orthogonal.

(b)

$$\begin{aligned} Qu &= (I - 2uu^T)u \\ &= Iu - 2uu^Tu \\ &= u - 2u(u^Tu) \\ &= u - 2u \\ &= -u \end{aligned}$$

$$\begin{aligned} Qv &= (I - 2uu^T)v \\ &= v - 2uu^Tv \\ &= v - 2u \langle v, u \rangle \\ &= v \end{aligned}$$

Suppose \hat{x} is the orthogonal projection of x onto $\text{span}\{u\}$, and $x_1 = x - \hat{x}$ and $x_2 = \hat{x} = \alpha u$. In this case, $(x - \hat{x}) \perp \hat{x} \Rightarrow x_1 \perp x_2$ and $x = x_1 + x_2$. Hence

$$Qx_2 = Q\hat{x} = \alpha Qu = -\alpha u = -x_2$$

$$Qx_1 = x_1$$

Hence

$$y = Qx = Q(x_1 + x_2) = x_1 - x_2$$

\hat{x} is the orthogonal projection of x onto $\text{span}\{u\}$. u is the normal vector of hyperplane $u^T x = 0$ and so x_1 should be the projection of x onto hyperplane $u^T x = 0$. Because $x = x_1 + x_2$ and $y = Qx = x_1 - x_2$, orthogonal projection of x onto $\text{span}\{u\}$ changes to negative but the projection of x onto hyperplane $u^T x = 0$ stay unchanged. So $y = Qx$ is actually reflect x through the hyperplane with normal vector u .

- (c) Known $Q \in \mathbb{R}^{n \times n}$, suppose u_1, u_2, \dots, u_n is the column of Q . Because Q is orthogonal, then u_1, u_2, \dots, u_n are orthogonal, hence u_1, u_2, \dots, u_n are linearly independent. Thus matrix Q is full-rank and invertible. Hence there is only one solution. Meanwhile

$$QQ = (I - 2uu^T)(I - 2uu^T) = Q$$

So

$$Qy = QQx = x$$

So the unique solution is $x = Qy$

- (d) Obviously matrix uu^T is square, hence

$$\det(Q) = \det(I - 2uu^T) = \det(I - 2u^T u I) = \det(I - 2I) = \det(-I) = -1$$

- (e) Following problem (b). Suppose \hat{x} is the orthogonal projection of x onto $\text{span}\{u\}$, and $x_1 = x - \hat{x}$ and $x_2 = \hat{x} = \alpha u$. Because $Qx \in y$, suppose $Qx = \beta y$. Hence we get

$$\begin{cases} x = x_1 + x_2 \\ \beta y = x_1 - x_2 \end{cases}$$

so we get

$$\begin{cases} x_1 = 0.5x + 0.5\beta y \\ x_2 = 0.5x - 0.5\beta y \end{cases}$$

Since $x_1 \perp x_2$, so

$$\langle 2x_1, 2x_2 \rangle = \langle x + \beta y, x - \beta y \rangle = \|x\|_2^2 - \beta^2 \|y\|_2^2 = 0$$

$$\Rightarrow \beta^2 = \frac{\|x\|_2^2}{\|y\|_2^2}$$

$$\Rightarrow x_2 = 0.5x - 0.5 \frac{\|x\|_2}{\|y\|_2} y$$

$$\Rightarrow u = \frac{x - \frac{\|x\|_2}{\|y\|_2} y}{\|x - \frac{\|x\|_2}{\|y\|_2} y\|_2}$$

If $0.5x - 0.5 \frac{\|x\|_2}{\|y\|_2} y = 0$, then any unit vector $u \perp x$ will make sense.

Problem 5: Projection Matrices

Solution

(a) Obviously $I - P$ is also a symmetric matrix.

$$\begin{aligned}(I - P)(I - P) &= (I - P) - P(I - P) \\ &= I - P - P + P^2 \\ &= I - 2P + P \\ &= I - P\end{aligned}$$

So $I - P$ is also a projection matrix.

(b) Obviously UU^T is symmetric matrix.

$$\begin{aligned}(UU^T)^2 &= UU^TUU^T \\ &= U(U^TU)U^T\end{aligned}$$

Because the columns of U is orthonormal, so $U^TU = I_{k \times k}$. Hence

$$(UU^T)^2 = U(U^TU)U^T = UIU^T = UU^T$$

So UU^T is a projection matrix.

(c) First we should show $P = A(A^TA)^{-1}A^T$ is a symmetric matrix.

$$\begin{aligned}[A(A^TA)^{-1}A^T]^T &= A[(A^TA)^{-1}]^TA^T \\ &= A[(A^TA)^T]^{-1}A^T \\ &= A(A^TA)^{-1}A^T\end{aligned}$$

So $A(A^TA)^{-1}A^T$ is a symmetric matrix. Second we should show that $P = P^2$.

$$\begin{aligned}P^2 &= A(A^TA)^{-1}A^TA(A^TA)^{-1}A^T \\ &= A(A^TA)^{-1}IA^T \\ &= A(A^TA)^{-1}A^T\end{aligned}$$

Hence $A(A^TA)^{-1}A^T$ is a projection matrix.

(d) Suppose $P = [p_1, p_2, \dots, p_n]$, where p_i is the column of matrix P . Hence $R(P)$ could be represented as $\text{span}\{p_1, p_2, \dots, p_n\}$. For any $p_i \in \{p_1, p_2, \dots, p_n\}$,

$$\langle x - y, p_i \rangle = p_i^T(x - Px) = (p_i^T - p_i^T P)x \quad (-6)$$

If P is a projection matrix, then $P = P^2$ and $P = P^T$ must be valid. Therefore,

$$P^2 = \begin{bmatrix} p_1^T p_1 & p_1^T p_2 & \cdots & p_1^T p_n \\ p_2^T p_1 & p_2^T p_2 & \cdots & p_2^T p_n \\ \vdots & \vdots & \ddots & \vdots \\ p_n^T p_1 & p_n^T p_2 & \cdots & p_n^T p_n \end{bmatrix} = \begin{bmatrix} \langle p_1, p_1 \rangle & \langle p_2, p_1 \rangle & \cdots & \langle p_n, p_1 \rangle \\ \langle p_1, p_2 \rangle & \langle p_2, p_2 \rangle & \cdots & \langle p_n, p_2 \rangle \\ \vdots & \vdots & \ddots & \vdots \\ \langle p_1, p_n \rangle & \langle p_2, p_n \rangle & \cdots & \langle p_n, p_n \rangle \end{bmatrix}$$

Hence

$$p_i = [\langle p_1, p_1 \rangle, \langle p_1, p_2 \rangle, \dots, \langle p_1, p_n \rangle]^T$$

Because $p_i \in \mathbb{R}^n$,

$$p_i = [\langle p_1, p_1 \rangle, \langle p_2, p_1 \rangle, \dots, \langle p_n, p_1 \rangle]^T$$

Using the result above into equation (1), then we get

$$p_i^T - p_i^T P = p_i^T - [\langle p_1, p_1 \rangle, \langle p_2, p_1 \rangle, \dots, \langle p_n, p_1 \rangle] = 0 \Rightarrow \langle x - y, p_i \rangle = 0$$

Hence y is the point in $R(P)$ closest to x . y is the projection of x . In conclusion, if P is a projection matrix, then $y = Px$ is the projection of x onto $R(P)$.

- (e) Obviously, the basis of $\text{span } u$ is $\{u\}$. Hence there is only one solution of the Normal Equation, that is:

$$\alpha = (u^T u)^{-1} u^T x$$

Therefore

$$y = u(u^T u)^{-1} u^T x \Rightarrow P = u(u^T u)^{-1} u^T = uu^T$$